Added auxiliary definitions for closed semantics

compcertxo/Lifting.v
@@ -4,40 +4,41 @@ Require Import Coqlib.
 Require Import LanguageInterface Events Globalenvs Smallstep.
 
 Section Lifting.
-  Variable abd: Type.
+  Variable K: Type.
   Definition lifted_li li: language_interface :=
     {|
-    query := query li * abd;
-    reply := reply li * abd;
+    query := query li * K;
+    reply := reply li * K;
     entry '(q, _) := entry q
     |}.
 
   Context {liA liB state} (L: lts liA liB state).
-  Let statex := (state * abd)%type.
-  Let liBx := lifted_li liB.
-  Let liAx := lifted_li liA.
+  Let stateX := (state * K)%type.
+  Let liBX := lifted_li liB.
+  Let liAX := lifted_li liA.
 
-  Inductive step' ge: statex -> trace -> statex -> Prop :=
+  Inductive step' ge: stateX -> trace -> stateX -> Prop :=
   | step'_intro: forall s s' a t,
       step L ge s t s' ->
       step' ge (s, a) t (s', a).
-  Inductive after_external': statex -> reply liAx -> statex -> Prop :=
+  Inductive after_external': stateX -> reply liAX -> stateX -> Prop :=
   | after_external'_intro: forall s a r a' s',
       after_external L s r s' ->
       after_external' (s, a) (r, a') (s, a').
 
-  Definition lifted_lts: lts liAx liBx statex :=
+  Definition lifted_lts: lts liAX liBX stateX :=
     {|
     genvtype := genvtype L;
     step ge := step' ge;
-    valid_query := fun (q: query liBx) => valid_query L (fst q);
+    valid_query := fun (q: query liBX) => valid_query L (fst q);
     initial_state := (initial_state L) * eq;
-    at_external := fun s (q: query liAx) => ((at_external L) * eq) s q;
+    at_external := fun s (q: query liAX) => ((at_external L) * eq) s q;
     after_external s := (after_external L (fst s)) * eq;
     final_state := (final_state L) * eq;
     globalenv := globalenv L
     |}%rel.
 End Lifting.
+
 
 Delimit Scope li_scope with li.
 Bind Scope li_scope with language_interface.
@@ -48,3 +49,142 @@ Bind Scope lts_scope with lts.
    precedence level will be inherited *)
 Notation "li @ K" := (lifted_li K li): li_scope.
 Notation "L @ K" := (lifted_lts K L): lts_scope.
+
+Definition lifted_semantics {liA liB} (K: Type) (L: semantics liA liB) :=
+  {|
+  skel := skel L;
+  activate se := (L se @ K)%lts;
+  |}.
+
+Delimit Scope sem_scope with sem.
+Bind Scope sem_scope with semantics.
+Notation "L @ K" := (lifted_semantics K L): sem_scope.
+
+Require Import Memory Values.
+
+Definition no_perm_on (m: mem) (vars: block -> Z -> Prop): Prop :=
+  forall b ofs, vars b ofs -> ~ Mem.perm m b ofs Max Nonempty.
+
+Record krel {K1 K2: Type}: Type :=
+  mk_krel {
+      Rk: K1 -> K2 -> Prop;
+      Rm: K1 -> mem -> Prop;
+      G: block -> Z -> Prop;
+
+      G_unchanged:
+        forall k m1 m2,
+          Rm k m1 -> Mem.unchanged_on G m1 m2 -> Rm k m2;
+    }.
+Arguments krel: clear implicits.
+
+Section SIM_REL.
+  Context {K1 K2} (R: krel K1 K2).
+
+  Inductive kcc_ext_query: query (li_c @ K1) -> query (li_c @ K2) -> Prop :=
+  | kcc_query_intro vf sg vargs1 vargs2 m1 m2 k1 k2:
+      Val.lessdef_list vargs1 vargs2 ->
+      Mem.extends m1 m2 ->
+      vf <> Vundef -> Rk R k1 k2 -> Rm R k1 m2 ->
+      no_perm_on m1 (G R) ->
+      kcc_ext_query (cq vf sg vargs1 m1, k1) (cq vf sg vargs2 m2, k2).
+
+  Inductive kcc_ext_reply: reply (li_c @ K1) -> reply (li_c @ K2) -> Prop :=
+  | kcc_ext_reply_intro vres1 vres2 m1 m2 k1 k2:
+      Val.lessdef vres1 vres2 ->
+      Mem.extends m1 m2 ->
+      Rk R k1 k2 -> Rm R k1 m2 ->
+      no_perm_on m1 (G R) ->
+      kcc_ext_reply (cr vres1 m1, k1) (cr vres2 m2, k2).
+
+  Program Definition kcc_ext :=
+    {|
+    ccworld := unit;
+    match_senv w := eq;
+    match_query w := kcc_ext_query;
+    match_reply w := kcc_ext_reply;
+    |}.
+
+End SIM_REL.
+
+Module Ksim.
+  Record ksim {K1 K2: Type} :=
+    mk_ksim {
+        L1: Smallstep.semantics li_null (li_c @ K1);
+        L2: Smallstep.semantics li_null (li_c @ K2);
+        R: krel K1 K2;
+
+        layer_sim: forward_simulation 1 (kcc_ext R) L1 L2;
+      }.
+  Arguments ksim: clear implicits.
+End Ksim.
+
+Definition lts_closed {liA liB} (L: semantics liA liB) :=
+  forall se s q, ~ (at_external (L se)) s q.
+
+Lemma li_null_closed {li} (L: semantics li_null li): lts_closed L.
+Proof.
+  unfold lts_closed.
+  intros. inversion q.
+Qed.
+
+Section LTS_CLOSED.
+
+  Context {liA liB} (L: semantics liA liB).
+  Context (HL: lts_closed L).
+
+  Variable liX: language_interface.
+  Definition lts' se: lts liX liB (state L) :=
+    {|
+    genvtype := genvtype (L se);
+    step ge := step (L se) ge;
+    valid_query := valid_query (L se);
+    initial_state := initial_state (L se);
+    at_external := fun s q => False;
+    after_external := fun q s r => False;
+    final_state := final_state (L se);
+    globalenv := globalenv (L se)
+    |}.
+  Definition closed_sem_conv :=
+    {|
+    skel := skel L;
+    activate se := lts' se;
+    |}.
+
+  (* TODO: proved equivalence *)
+End LTS_CLOSED.
+
+Require Import Clight.
+Require Import CatComp.
+Require Import Linking.
+
+Definition layer_combine {K} (M: Clight.program)
+           (L: Smallstep.semantics li_null (li_c @ K)) sk :=
+  let L' := CatComp.semantics (semantics1 M @ K) (closed_sem_conv L (li_c @ K)) sk
+  in closed_sem_conv L' li_null.
+
+
+Record prog_ksim {K1 K2: Type} :=
+  mk_prog_ksim {
+      L1: Smallstep.semantics li_null (li_c @ K1);
+      L2: Smallstep.semantics li_null (li_c @ K2);
+      M: Clight.program;
+      R: krel K1 K2;
+      sk: AST.program unit unit;
+
+      layer_sim: forward_simulation 1 (kcc_ext R) L1 (layer_combine M L2 sk);
+      link_sk: link (skel (semantics1 M)) (skel L2) = Some sk;
+    }.
+
+Section PROG_SIM.
+  Context {K1 K2} (pksim: @prog_ksim K1 K2).
+  Program Definition prog_sim_coercion: @Ksim.ksim K1 K2 :=
+    {|Ksim.L1 := L1 pksim;
+      Ksim.L2 := layer_combine (M pksim) (L2 pksim) (sk pksim);
+      Ksim.R := R pksim; |}.
+  Next Obligation.
+    exact (layer_sim pksim).
+  Qed.
+End PROG_SIM.
+Coercion prog_sim_coercion : prog_ksim >-> Ksim.ksim.
+
+Require Import FlatComp.
